Auto/Lib/IntExtra.lean
@@ -1,16 +1,17 @@
+import Auto.Lib.NatExtra
 namespace Auto
-
--- A version of `Nat.beq_refl` that reduces to `Eq.refl`
-def Nat.beq_refl' : (a : Nat) → (a.beq a) = true
-| 0 => rfl
-| n + 1 => Nat.beq_refl' n
 
 def Int.beq : Int → Int → Bool
 | .ofNat n₁,   .ofNat n₂   => n₁.beq n₂
 | .negSucc n₁, .negSucc n₂ => n₁.beq n₂
 | _,           _           => false
 
-def Int.beq_refl : (i : Int) → (Int.beq i i) = true
+instance : BEq Int where
+  beq := Int.beq
+
+theorem Int.beq_def {a b : Int} : (a == b) = Int.beq a b := rfl
+
+def Int.beq_refl : {i : Int} → (Int.beq i i) = true
 | .ofNat n => Nat.beq_refl' n
 | .negSucc n => Nat.beq_refl' n
 
@@ -20,5 +21,9 @@ def Int.eq_of_beq_eq_true {i₁ i₂ : Int} : Int.beq i₁ i₂ → i₁ = i₂ 
   | .negSucc n₁, .negSucc n₂ => fun H => congrArg _ (Nat.eq_of_beq_eq_true H)
   | .ofNat n₁, .negSucc n₂ => fun H => by cases H
   | .negSucc n₁, .ofNat n₂ => fun H => by cases H
+
+instance : LawfulBEq Int where
+  eq_of_beq := Int.eq_of_beq_eq_true
+  rfl := Int.beq_refl
 
 end Auto
