Auto/Lib/BoolExtra.lean
@@ -1,11 +1,5 @@
 namespace Auto
 
-theorem Bool.beq_refl {a : Bool} : a == a := by
-  cases a <;> rfl
-
-theorem Bool.eq_of_beq_eq_true {a b : Bool} (h : a == b) : a = b := by
-  cases a <;> cases b <;> cases h <;> rfl
-
 theorem Bool.eq_false_of_ne_true {a : Bool} : a ≠ true → a = false := by
   cases a <;> decide
 
